Environments flushed out

lean/Cyclone_Formal_Syntax.lean
@@ -9,8 +9,6 @@ inductive Kappa : Type
 | A    /- 'any'   kind. -/
 export Kappa
 
-#print Kappa
-
 inductive Phi : Type
 | witnesschanges /- Allowing witness changes. \delta -/
 | aliases        /- Allowing aliases as the opened type. \amp -/ 
@@ -26,79 +24,80 @@ export IPE
 
 @[derive decidable_eq]
 inductive PE : Type 
-| i_pe      : IPE -> PE
+| i_pe      : IPE → PE
 | u_pe      : PE
 
 export PE 
 
+notation `Var`     := string
+
 inductive V : Type
-| bevar : nat -> V     /- A bound expression variable, a de Bruijn index. -/
-| fevar : string -> V  /- A free expression variable. -/
+| bevar : nat → V     /- A bound expression variable, a de Bruijn index. -/
+| fevar : Var → V  /- A free expression variable. -/
 
 export V
 
-mutual inductive St, E, F, Tau 
-with St : Type 
- | e_s       : E   -> St                 /- An expression in a statement. -/
- | retn      : E   -> St                 /- Returns are required in this syntax. -/
- | seqx      : St  -> St -> St           /- Statement sequencing. -/
- | if_s      : E   -> St -> St   -> St   /- if expression in a statement. -/
- | while     : E   -> St -> St           /- A while statement. -/
- | letx      : E   -> St -> St           /- A let expression. -/
- | openx     : E   -> St -> St           /- open an existential package (elimination) to a value. -/
- | openstar  : E   -> St -> St           /- open an existential package (elimination) with a pointer to the value. -/
-with E : Type                            /- Terms for expressions. -/
- | v_e        : V -> E                   /- Put a variable into an expression, either bound or free. -/
- | i_e        : ℤ -> E                   /- An integer value in an expression. -/
- | p_e        : V -> list PE -> E        /- This is a term that derefences a path into the value of the variable. -/
- | f_e        : F -> E                   /- A function identifier in an expression or statement. -/
- | amp        : E -> E                   /- Take the address of an expression. -/
- | star       : E -> E                   /- Derefence an expression of a pointer type. -/
- | cpair      : E -> E -> E              /- A pair in an expression. -/
- | dot        : E -> IPE -> E            /- A deference of a pair. -/
- | assign     : E -> E -> E              /- Assignment. -/
- | appl       : E -> E -> E              /- Application expression. app is append. -/
- | call       : St -> E                  /- A call expression for the semantics use. -/
- | inst       : E -> Tau -> E            /- Type instantiation, e[\tau]. -/
- | pack       : Tau -> E -> Tau -> E     /- Existential type introduction. -/
-/- This was done in Coq to make induction work, perhaps it works without it? -/
-with F : Type 
- | dfun       : Tau -> Tau -> St -> F    /- Function definition. -/
- | ufun       : Kappa -> F -> F          /- Univerally quantified polymorphic function definition.  -/
-with Tau : Type
- | btvar  : nat -> Tau                   /- A bound type variable, a de Bruijn index. -/
- | ftvar  : string -> Tau                /- A free type variable. -/
- | cint   : Tau                          /- Cyclone's Integers. -/
- | cross  : Tau -> Tau -> Tau            /- Pairs. -/
- | arrow  : Tau -> Tau -> Tau            /- Function    type. -/
- | ptype  : Tau -> Tau                   /- Pointer     type. -/
+inductive Tau : Type
+ | btvar  : nat → Tau                /- A bound type variable, a de Bruijn index. -/
+ | ftvar  : Var → Tau                /- A free type variable. -/
+ | cint   : Tau                      /- Cyclone's Integers. -/
+ | cross  : Tau → Tau → Tau          /- Pairs. -/
+ | arrow  : Tau → Tau → Tau          /- Function    type. -/
+ | ptype  : Tau → Tau                /- Pointer     type. -/
 /-
- | utype  : Kappa -> Tau -> Tau          /- Universal   type. -/
- | etype  : Phi -> Kappa -> Tau -> Tau   /- Existential type. -/
+ | utype  : Kappa → Tau → Tau        /- Universal   type. -/
+ | etype  : Phi → Kappa → Tau → Tau  /- Existential type. -/
 -/
+export Tau
+
+mutual inductive St, E, F
+with St : Type 
+ | e_s       : E   → St              /- An expression in a statement. -/
+ | retn      : E   → St              /- Returns are required in this syntax. -/
+ | seqx      : St  → St → St         /- Statement sequencing. -/
+ | if_s      : E   → St → St   → St  /- if expression in a statement. -/
+ | while     : E   → St → St         /- A while statement. -/
+ | letx      : E   → St → St         /- A let expression. -/
+ | openx     : E   → St → St         /- open an existential package (elimination) to a value. -/
+ | openstar  : E   → St → St         /- open an existential package (elimination) with a pointer to the value. -/
+with E : Type                        /- Terms for expressions. -/
+ | v_e        : V → E                /- Put a variable into an expression, either bound or free. -/
+ | i_e        : ℤ → E                /- An integer value in an expression. -/
+ | p_e        : V → list PE → E      /- This is a term that derefences a path into the value of the variable. -/
+ | f_e        : F → E                /- A function identifier in an expression or statement. -/
+ | amp        : E → E                /- Take the address of an expression. -/
+ | star       : E → E                /- Derefence an expression of a pointer type. -/
+ | cpair      : E → E → E            /- A pair in an expression. -/
+ | dot        : E → IPE → E          /- A deference of a pair. -/
+ | assign     : E → E → E            /- Assignment. -/
+ | appl       : E → E → E            /- Application expression. app is append. -/
+ | call       : St → E               /- A call expression for the semantics use. -/
+ | inst       : E → Tau → E          /- Type instantiation, e[\tau]. -/
+ | pack       : Tau → E → Tau → E    /- Existential type introduction. -/
+with F : Type 
+ | dfun       : Tau → Tau → St → F    /- Function definition. -/
+ | ufun       : Kappa → F → F         /- Univerally quantified polymorphic function definition.  -/
 
 export St
 export E 
 export F 
-export Tau
 
 inductive Term : Type
-| term_st : St -> Term 
-| term_e :  E -> Term 
-| term_f :  F -> Term
+| term_st : St → Term 
+| term_e :  E → Term 
+| term_f :  F → Term
 export Term
 
-inductive Value : E -> Prop
+inductive Value : E → Prop
 | IIsAValue    : forall (i : ℤ), Value (E.i_e i)
-| AmpIsAValue  : forall (v : string) (p : list PE),  Value (amp (E.p_e (V.fevar v) p)) 
+| AmpIsAValue  : forall (v : Var) (p : list PE),  Value (amp (E.p_e (V.fevar v) p)) 
 | DfunIsAValue : forall (t1 t2 : Tau) (s : St), Value (E.f_e (F.dfun t1 t2 s))
 | UfunIsAValue : forall (k : Kappa) (f : F),    Value (E.f_e (F.ufun k f))
-| PairIsAValue : forall (v0 v1 : E), Value v0 -> Value v1 -> Value (E.cpair v0 v1)
-| PackIsAValue : forall (tau tau': Tau) (v : E), Value v -> Value (E.pack tau v tau')
+| PairIsAValue : forall (v0 v1 : E), Value v0 → Value v1 → Value (E.cpair v0 v1)
+| PackIsAValue : forall (tau tau': Tau) (v : E), Value v → Value (E.pack tau v tau')
 
-notation `Var`     := string
 notation `Path`    := list PE
-notation `Binding` := string × E 
+notation `Binding` := Var × E 
 notation `Heap`    := list Binding
 notation `State`   := Heap × St
 notation `Delta`   := list (Var × Kappa) 
