lean/Cyclone_Static_Semantics_Kinding_And_Context_Well_Formedness.lean
@@ -1,4 +1,4 @@
-/- 
+/-
  This is the definition of formal syntax for Dan Grossman's Thesis, 
   "SAFE PROGRAMMING AT THE C LEVEL OF ABSTRACTION". 
 
@@ -8,13 +8,14 @@
 import .Cyclone_Formal_Syntax
 import .Environments
 
+/- This is nothing but ok. -/
 inductive WFD : Delta → Prop
 | empty : WFD []
 | xtau   : ∀ (d : Delta) (alpha : Var) (k : Kappa),
-            binds alpha d = none →
+            binds alpha d none →
             ok d →
             WFD  d →
-            WFD (d ++ [(alpha, k)])
+            WFD ((alpha, k) :: d)
 
 @[simp] lemma WFD_empty : 
   WFD [] := 
@@ -27,26 +28,30 @@ begin
  simp, 
 end
 
-inductive K : Delta → Tau → Kappa → Prop 
+inductive K : Delta → Tau -> Kappa → Prop
  | cint   : ∀ (d : Delta), K d cint B
  | B      : ∀ (alpha : Var) (d : Delta),
-               binds alpha d = some B →
+               binds alpha d (some B) →
                K d (ftvar alpha) B
  | star_A  : ∀ (alpha : Var) (d : Delta), 
-                 binds alpha d = some A → 
+                 binds alpha d (some A) → 
                  K  d (ptype (ftvar alpha)) B
- | cross   : forall (d : Delta) (t0 t1 : Tau),
+ | cross   : ∀ (d : Delta) (t0 t1 : Tau),
                     K d t0 A →
                     K d t1 A →
                     K d (cross t0 t1) A
- | arrow   : forall (d : Delta) (t0 t1 : Tau),
+ | arrow   : ∀ (d : Delta) (t0 t1 : Tau),
                     K d t0 A →
                     K d t1 A →
                     K d (arrow t0 t1) A
 
- | ptype   : forall (d : Delta) (tau : Tau),
+ | ptype   : ∀ (d : Delta) (tau : Tau),
                     K d tau A →
                     K d (ptype tau) B
+
+ | B_A     : ∀ (d : Delta) (tau : Tau),
+              K d tau B →
+              K d tau A
 /-
  | utype  : forall (L : set Var) (d : Delta) (k : Kappa) (tau : Tau),
             (forall (alpha : Var),
@@ -61,43 +66,42 @@ inductive K : Delta → Tau → Kappa → Prop
                 K (d & alpha ~ k) (T.open_rec 0 (ftvar alpha) tau) A) →
               K d (etype p k tau) A
 -/
- | B_A     : forall (d : Delta) (tau : Tau),
-              K d tau B →
-              K d tau A
+
+
 
 inductive AK : Delta → Tau → Kappa → Prop
- | AAK  : forall (d : Delta) (tau : Tau) (k : Kappa),
+ | AAK  : ∀ (d : Delta) (tau : Tau) (k : Kappa),
            K  d tau k →
            AK d tau k
- | AA   : forall (d : Delta) (alpha : Var),
-           binds alpha d = some A → 
+ | AA   : ∀ (d : Delta) (alpha : Var),
+           binds alpha d (some A) → 
            AK d (ftvar alpha) A
 
 inductive ASGN : Delta → Tau → Prop
-  | ASGN_cint  : forall (d : Delta),
+  | ASGN_cint  : ∀ (d : Delta),
                       ASGN d cint
-  | ASGN_B     : forall (d : Delta) (alpha : Var),
-                   binds alpha d = some B →
+  | ASGN_B     : ∀ (d : Delta) (alpha : Var),
+                   binds alpha d (some B) →
                    ASGN d (ftvar alpha)
-  | ASGN_ptype : forall (d : Delta) (tau : Tau),
+  | ASGN_ptype : ∀ (d : Delta) (tau : Tau),
                    ASGN d (ptype tau)
-  | ASGN_cross : forall (d : Delta) (t0 t1 : Tau),
+  | ASGN_cross : ∀ (d : Delta) (t0 t1 : Tau),
                    ASGN d t0 → 
                    ASGN d t1 → 
                    ASGN d (cross t0 t1)
-  | ASGN_arrow : forall (d : Delta) (t0 t1 : Tau),
+  | ASGN_arrow : ∀ (d : Delta) (t0 t1 : Tau),
                    ASGN d t0 → 
                    ASGN d t1 → 
                    ASGN d (arrow t0 t1)
 /-
-  | ASGN_utype : forall (L : Vars) (d : Delta)  (k : Kappa) (tau : Tau),
-                 (forall (alpha : Var),
+  | ASGN_utype : ∀ (L : Vars) (d : Delta)  (k : Kappa) (tau : Tau),
+                 (∀ (alpha : Var),
                    alpha \notin L →
                    ASGN (d & alpha ~ k) (T.open_rec 0 (ftvar alpha) tau)) →
                    ASGN d (utype k tau)
 
-  | ASGN_etype : forall (L : Vars) (d : Delta) (k : Kappa) (tau : Tau),
-                 (forall (alpha : Var),
+  | ASGN_etype : ∀ (L : Vars) (d : Delta) (k : Kappa) (tau : Tau),
+                 (∀ (alpha : Var),
                    alpha \notin L →
                    ASGN (d & alpha ~ k) (T.open_rec 0 (ftvar alpha) tau)) →
                    ASGN d (etype witnesschanges k tau)
@@ -105,28 +109,27 @@ inductive ASGN : Delta → Tau → Prop
 
 inductive WFU : Upsilon → Prop 
   | empty : WFU []
-  | A   : forall (u : Upsilon) (tau : Tau) (p : Path) (x : Var),
+  | A   : ∀ (u : Upsilon) (tau : Tau) (p : Path) (x : Var),
            ok u →
-           binds (x,p) u = none →
+           binds (x,p) u none →
            WFU  u →
            K [] tau A →
-           WFU (u ++ [((x,p),tau)])
+           WFU (((x,p),tau) :: u)
 
 inductive WFDG : Delta → Gamma → Prop 
-  | d_empty : forall (d: Delta),
+  | d_empty : ∀ (d: Delta),
                      ok d →
                      WFDG d []
-  | xt      : forall (d: Delta) (g: Gamma) (x : Var) (tau : Tau),
+  | xt      : ∀ (d: Delta) (g: Gamma) (x : Var) (tau : Tau),
                      ok g →
                      ok d →
-                     binds x g = none → 
+                     binds x g none → 
                      K d tau A →
                      WFDG d g →
-                     WFDG d (g ++ [(x, tau)])
+                     WFDG d ((x, tau) :: g)
 
 inductive WFC : Delta → Upsilon → Gamma → Prop 
-  | DUG : forall (d : Delta) (g: Gamma) (u : Upsilon),
+  | DUG : ∀ (d : Delta) (g: Gamma) (u : Upsilon),
                 WFDG d g →
                 WFU u →
                 WFC d u g
-
