lean/Cyclone_K_lemmas.lean
@@ -1,0 +1,295 @@
+/-
+ This is the definition of formal syntax for Dan Grossman's Thesis, 
+  "SAFE PROGRAMMING AT THE C LEVEL OF ABSTRACTION". 
+
+   Some K Lemmas.
+-/
+/- These are missing utype and etype. -/
+
+import .Cyclone_Static_Semantics_Kinding_And_Context_Well_Formedness
+
+lemma K_weakening (t : Tau) (d : Delta) :
+ K d t A →
+ WFD d →
+ ∀ (d' : Delta),
+  extendedby d d' →
+  K d' t A :=
+begin
+ intros kdta wfdd d extdd',
+ induction kdta,
+/- This would be nicer if I had disjunctive cases.
+ try {solve1{constructor}};
+ try {constructor,
+      apply binds_extendedby,
+      repeat {assumption}, };
+ try {constructor,
+     apply kdta_ih_a,
+     repeat {assumption,},
+     apply kdta_ih_a_1,
+     repeat {assumption,},};
+ try {constructor,
+     apply kdta_ih,
+     repeat{ assumption, },},
+-/
+ case K.cint {
+   constructor,
+ },
+ case K.B { 
+   constructor,
+   apply binds_extendedby; assumption,
+},
+ case K.star_A {
+   constructor,
+   apply binds_extendedby; assumption},
+ case K.cross {
+    constructor,
+    apply kdta_ih_a; assumption,
+    apply kdta_ih_a_1; assumption, 
+ },
+ case K.arrow {
+    constructor,
+    apply kdta_ih_a; assumption,
+    apply kdta_ih_a_1; assumption,
+ },
+ case K.ptype    { 
+   constructor,
+   apply kdta_ih; assumption,
+},
+ case K.B_A {
+  constructor,
+  apply kdta_ih; assumption,
+},
+end
+
+lemma K_weakening_var (d : Delta) (t : Tau) (k : Kappa) :
+ ok d →
+ K d t k →
+ ∀ (v : Var) (k' : Kappa),
+   ok ((v,k') :: d) →
+   K  ((v,k') :: d) t k :=
+begin
+  intros okd kdtk,
+  induction' kdtk; 
+  intros v k' okvk';
+  try {solve1 {constructor} };
+  try {
+   constructor,
+   apply binds_weakening; 
+   assumption};
+  try{
+   constructor;
+   try {apply ih; assumption},
+   try {apply ih_kdtk; assumption},
+   try {apply ih_kdtk_1; assumption},
+ },
+end
+
+/- WTF? it's not putting the A of A -> false in the context. -/
+lemma bug :
+   ¬ false :=
+begin
+   intros v,
+   assumption,
+end
+
+lemma K_empty_var (v : Var) (k : Kappa) :
+   ¬ K [] (ftvar v) k :=
+begin
+  intros k,
+  cases k; cases k_a,
+  apply binds_nil_not_some v B; assumption,
+end
+
+/-
+
+lemma open_var_fv_eq : ∀ t n x,
+    T.fv (T.open_rec n (ftvar x) t) = (T.fv t \u \{x}) \/
+    T.fv (T.open_rec n (ftvar x) t) = (T.fv t).
+Proof.
+  intros t.
+  induction t; intros; simpl; try case_nat; auto with fset;
+  try solve[
+        simpl;
+        left;
+        rewrite union_empty_l;
+        auto with fset].
+(* Bug ugly won't ltac. *)
+
+  specialize(IHt1 n x);
+  specialize(IHt2 n x);
+  inversion IHt1; inversion IHt2;
+  rewrite H; rewrite H0.
+  left.
+  rewrite <- union_assoc.
+  rewrite <- union_assoc.
+  rewrite* union_middle_shuffle.
+  left.
+  rewrite <- union_assoc.
+  rewrite <- union_assoc.
+  rewrite* union_middle_r.
+  left.
+  rewrite* <- union_assoc.  
+  right*.
+
+  specialize(IHt1 n x);
+  specialize(IHt2 n x);
+  inversion IHt1; inversion IHt2;
+  rewrite H; rewrite H0.
+  left.
+  rewrite <- union_assoc.
+  rewrite <- union_assoc.
+  rewrite* union_middle_shuffle.
+  left.
+  rewrite <- union_assoc.
+  rewrite <- union_assoc.
+  rewrite* union_middle_r.
+  left.
+  rewrite* <- union_assoc.  
+  right*.  
+Qed.  
+
+lemma fv_var:
+  ∀ A alpha tau (d : env A), 
+    alpha \notin T.fv tau →
+    T.fv tau \c \{ alpha} \u dom d →
+    T.fv tau \c dom d.
+Proof.
+  intros.
+  induction tau; simpl; simpl in H; simpl in H0; auto with fset.
+  assert(alpha <> v); auto.
+  lets: subset_remove_r (fset Tau).
+  apply subset_remove_r with (b:= alpha); auto.
+  assert(alpha \notin T.fv tau1); auto.
+  assert(alpha \notin T.fv tau2); auto.
+  specialize (IHtau1 H1).
+  specialize (IHtau2 H2).
+  assert(H3 : (T.fv tau1 \u T.fv tau2 \c \{ alpha} \u dom d)); auto.
+  apply subset_remove_l_r in H0.  
+  apply subset_remove_l_l in H3.
+  auto with fset.
+
+  assert(H3 : (T.fv tau1 \u T.fv tau2 \c \{ alpha} \u dom d)); auto.
+  apply subset_remove_l_r in H0.  
+  apply subset_remove_l_l in H3.
+  auto with fset.  
+Qed.  
+
+lemma fv_var_2:
+  ∀ A alpha tau (d : env A), 
+    alpha \notin T.fv tau →
+    T.fv tau \u \{ alpha} \c \{ alpha} \u dom d →
+    T.fv tau \c dom d.
+Proof.
+  intros.
+  apply subset_remove_l_r in H0.
+  apply fv_var with (alpha:= alpha); auto.
+Qed.
+
+lemma K_fv:
+  ∀ tau d k,
+    WFD d →
+    K d tau k →
+    T.fv tau \c fv_delta d.
+Proof.
+(* BUG ugly, repetition, will not ltac *)
+  introv WFDd Kd.
+  induction Kd; assert(ok d); auto; try solve[simpl; auto with fset].
+
+  pick_fresh alpha.
+  assert(NI: alpha \notin L); auto.
+  assert(OKda: ok(d & alpha ~ k)); auto.
+  assert(WFDda: WFD(d & alpha ~k)); auto.
+  specialize (H0 alpha NI OKda WFDda).
+  lets: open_var_fv_eq tau 0 alpha.
+  inversion H2.
+  rewrite H3 in H0.
+  unfold fv_delta.
+  unfold fv_delta in H0.
+  rewrite dom_push in H0.
+  apply fv_var_2 with (alpha:=alpha); auto.
+  rewrite H3 in H0.
+  unfold fv_delta in H0.
+  unfold fv_delta.
+  apply fv_var with (alpha:= alpha); auto.
+  unfold fv_delta in H0.
+  unfold fv_delta.
+  rewrite dom_push in H0.
+  auto.  
+
+  pick_fresh alpha.
+  assert(NI: alpha \notin L); auto.
+  assert(OKda: ok(d & alpha ~ k)); auto.
+  assert(WFDda: WFD(d & alpha ~k)); auto.
+  specialize (H0 alpha NI OKda WFDda).
+  lets: open_var_fv_eq tau 0 alpha.
+  inversion H2.
+  rewrite H3 in H0.
+  unfold fv_delta.
+  unfold fv_delta in H0.
+  rewrite dom_push in H0.
+  apply fv_var_2 with (alpha:=alpha); auto.
+  rewrite H3 in H0.
+  unfold fv_delta in H0.
+  unfold fv_delta.
+  apply fv_var with (alpha:= alpha); auto.
+  unfold fv_delta in H0.
+  unfold fv_delta.
+  rewrite dom_push in H0.
+  auto.  
+Qed.
+
+lemma K_empty_closed:
+  ∀ tau k,
+    K empty tau k →
+    T.fv tau = \{}.
+Proof.
+  intros.
+  lets: K_fv tau (@empty Kappa).
+  apply H0 in H.
+  unfold fv_delta in H.
+  rewrite dom_empty in H.
+  apply contained_in_empty in H; auto.
+  auto.
+Qed.
+
+lemma K__lc:
+  ∀ d t k,
+    ok d →
+    K d t k →
+    T.lc t.
+Proof.
+  introv okd Kd.
+  induction Kd; auto.
+  apply_fresh T.lc_utype.
+  assert(NI: y \notin L); auto.
+  apply_fresh T.lc_etype.
+  assert(NI: y \notin L); auto.
+Qed.
+
+lemma AK_weakening_k:
+  ∀ tau d k,
+    AK d tau k →
+    ∀ d',
+      WFD d →
+      extends d d' →
+      AK d' tau k.
+Proof.
+  introv AKd.
+  induction AKd; try solve[auto].
+  intros.
+  constructor.
+  apply K_weakening_k with (d:=d); auto.
+Qed.  
+
+lemma AK_weakening_var:
+  ∀ d t k,
+    ok d →
+    AK d t k →
+    ∀ alpha k',
+      ok (d & alpha ~ k') →
+      AK (d & alpha ~ k') t k.
+Proof.
+  intros.
+  apply AK_weakening_k with (d:= d); auto.
+Qed.
+-/
